feat: verify `all` and `any` for hash maps (#10765)
This PR extends the `all`/`any` functions from hash sets to hash maps
and dependent hash maps and verifies them.

src/Std/Data/DHashMap/Raw.lean
@@ -487,6 +487,17 @@ only those mappings where the function returns `some` value.
 @[inline] def keysArray (m : Raw α β) : Array α :=
   m.fold (fun acc k _ => acc.push k) (.emptyWithCapacity m.size)
 
+/-- Checks if all elements satisfy the predicate, short-circuiting if a predicate fails. -/
+@[inline] def all (m : Raw α β) (p : (a : α) → β a → Bool) : Bool := Id.run do
+  for a in m do
+    if ¬ p a.1 a.2 then return false
+  return true
+
+/-- Checks if any element satisfies the predicate, short-circuiting if a predicate succeeds. -/
+@[inline] def any (m : Raw α β) (p : (a : α) → β a → Bool) : Bool := Id.run do
+  for a in m do
+    if p a.1 a.2 then return true
+  return false
 /--
 Computes the union of the given hash maps. If a key appears in both maps, the entry contained in
 the second argument will appear in the result.
