src/Std/Data/HashSet/Lemmas.lean
@@ -557,6 +557,60 @@ theorem forIn_eq_forIn_toArray [Monad m'] [LawfulMonad m']
 
 end monadic
 
+theorem all_eq_not_any_not {p : α → Bool} :
+    m.all p = ! m.any (fun a => ! p a) := HashMap.all_eq_not_any_not
+
+theorem any_eq_not_all_not {p : α → Bool} :
+    m.any p = ! m.all (fun a => ! p a) := HashMap.any_eq_not_all_not
+
+@[simp]
+theorem any_toList [LawfulHashable α] [EquivBEq α] {p : α → Bool} :
+    m.toList.any p = m.any p :=
+  HashMap.any_keys
+
+theorem any_eq_true_iff_exists_mem_get [LawfulHashable α] [EquivBEq α]
+    {p : α → Bool} :
+    m.any p = true ↔ ∃ (a : α) (h : a ∈ m), p (m.get a h) :=
+  HashMap.any_eq_true_iff_exists_mem_getKey_getElem
+
+theorem any_eq_true_iff_exists_mem [LawfulBEq α] {p : α → Bool} :
+    m.any p = true ↔ ∃ (a : α), a ∈ m ∧ p a := by
+  simpa using @HashMap.any_eq_true_iff_exists_mem_getElem _ _ _ _ _ _ (fun a b => p a)
+
+theorem any_eq_false_iff_forall_mem_get [LawfulHashable α] [EquivBEq α]
+    {p : α → Bool} :
+    m.any p = false ↔
+      ∀ (a : α) (h : a ∈ m), p (m.get a h) = false :=
+  HashMap.any_eq_false_iff_forall_mem_getKey_getElem
+
+theorem any_eq_false_iff_forall_mem [LawfulBEq α] {p : α → Bool} :
+    m.any p = false ↔
+      ∀ (a : α), a ∈ m → p a = false := by
+  simpa using @HashMap.any_eq_false_iff_forall_mem_getElem _ _ _ _ _ _ (fun a b => p a)
+
+@[simp]
+theorem all_toList [LawfulHashable α] [EquivBEq α] {p : α → Bool} :
+    m.toList.all p =m.all p :=
+  HashMap.all_keys
+
+theorem all_eq_true_iff_forall_mem_get [EquivBEq α] [LawfulHashable α]
+    {p : α → Bool} :
+    m.all p = true ↔ ∀ (a : α) (h : a ∈ m), p (m.get a h) :=
+  HashMap.all_eq_true_iff_forall_mem_getKey_getElem
+
+theorem all_eq_true_iff_forall_mem [LawfulBEq α] {p : α → Bool} :
+    m.all p = true ↔ ∀ (a : α), a ∈ m → p a :=
+  HashMap.all_eq_true_iff_forall_mem_getElem
+
+theorem all_eq_false_iff_exists_mem_get [EquivBEq α] [LawfulHashable α]
+    {p : α → Bool} :
+    m.all p = false ↔ ∃ (a : α) (h : a ∈ m), p (m.get a h) = false :=
+  HashMap.all_eq_false_iff_exists_mem_getKey_getElem
+
+theorem all_eq_false_iff_exists_mem [LawfulBEq α] {p : α → Bool} :
+    m.all p = false ↔ ∃ (a : α), a ∈ m ∧ p a = false := by
+  simpa using @HashMap.all_eq_false_iff_exists_mem_getElem _ _ _ _ _ _ (fun a b => p a)
+
 variable {ρ : Type v} [ForIn Id ρ α]
 
 @[simp, grind =]
